Logos/Prelude.lean
@@ -1,2 +1,3 @@
 import Logos.Prelude.Newtype
 import Logos.Prelude.FunTypes
+import Logos.Prelude.NatLit
