Logos/Prelude/NatLit.lean
@@ -1,0 +1,75 @@
+import Logos.Prelude.Newtype
+import Logos.Prelude.FunTypes
+
+universe u
+variable {T : Sort u}
+
+namespace Logos
+
+/--
+  Sort-polymorphic Natural Literals
+-/
+class OfNatLit (A : Sort u) (n : Nat) :=
+  ofNatLit : A
+
+@[defaultInstance low]
+instance iNatOfNatLit {n : Nat} : OfNatLit Nat n
+  := {ofNatLit := n}
+
+@[defaultInstance low + low]
+instance iOfNatLitOfNat {A : Type u} {n : Nat} 
+  [K : OfNat A n] : OfNatLit A n
+  := {ofNatLit := K.ofNat}
+
+instance iOfMatOfNatLit {A : Type u} {n : Nat} 
+  [K : OfNatLit A n] : OfNat A n
+  := {ofNat := K.ofNatLit}
+
+-- 0
+
+class abbrev Zero (T : Sort u) 
+  := OfNatLit T (nat_lit 0)
+
+instance Zero.isNewtype : Newtype (Zero T) T :=
+  {pack := fun x => {ofNatLit := x}, unpack := fun K => K.ofNatLit}
+
+instance Zero.ofNat : Zero Nat := 
+  {ofNatLit := Nat.zero}
+
+-- 1
+
+class abbrev One (T : Sort u) 
+  := OfNatLit T (nat_lit 1)
+
+instance One.isNewtype : Newtype (Zero T) T :=
+  {pack := fun x => {ofNatLit := x}, unpack := fun K => K.ofNatLit}
+
+instance One.ofNat : One Nat := 
+  {ofNatLit := Nat.succ Nat.zero}
+
+-- S
+
+class funtype Succ (T : Sort u) : Unar T
+
+abbrev S [K : Succ T] := K.toFun
+
+instance Succ.ofNat : Succ Nat := pack Nat.succ
+instance Succ.ofNatLit {A : Sort u} [K : Succ A] (n : Nat) [T : OfNatLit A n] 
+  : OfNatLit A (Nat.succ n) := {ofNatLit := unpack K T.ofNatLit}
+
+namespace Notation
+
+open Lean
+
+scoped syntax:max (name := sortNumLit) (priority := default + default) 
+  num : term
+
+@[macro sortNumLit] 
+def expandSortNumLit : Macro
+  | `( $n:numLit ) => `(OfNatLit.ofNatLit (nat_lit $n))
+  | _ => Macro.throwUnsupported
+
+@[scoped appUnexpander Logos.OfNatLit.ofNatLit] 
+def unexpandOfNatLit : PrettyPrinter.Unexpander
+  | `($_f:ident $n:numLit) => n
+  | _  => throw ()
